Weidenbach_Book/CDCL_Conflict_Minimisation.thy
@@ -411,79 +411,6 @@ definition lit_redundant_rec_spec where
     SPEC(\<lambda>(cach, analysis, b). (b \<longrightarrow> NU \<Turnstile>pm add_mset (-L) (filter_to_poslev M L D)) \<and>
      conflict_min_analysis_inv M cach NU D)\<close>
 
-(* TODO Move *)
-context conflict_driven_clause_learning\<^sub>W
-begin
-
-lemma in_unmark_l_in_lits_of_l_iff: \<open>{#L#} \<in> unmark_l M \<longleftrightarrow> L \<in> lits_of_l M\<close>
-  by (induction M) auto
-
-lemma literals_of_level0_entailed:
-  assumes
-    struct_invs: \<open>cdcl\<^sub>W_all_struct_inv S\<close> and
-    in_trail: \<open>L \<in> lits_of_l (trail S)\<close> and
-    lev: \<open>get_level (trail S) L = 0\<close>
-  shows
-    \<open>clauses S \<Turnstile>pm {#L#}\<close>
-proof -
-  have decomp: \<open>all_decomposition_implies_m (clauses S) (get_all_ann_decomposition (trail S))\<close>
-    using struct_invs unfolding cdcl\<^sub>W_all_struct_inv_def
-    by fast
-  have L_trail: \<open>{#L#} \<in> unmark_l (trail S)\<close>
-    using in_trail by (auto simp: in_unmark_l_in_lits_of_l_iff)
-  have n_d: \<open>no_dup (trail S)\<close>
-    using struct_invs unfolding cdcl\<^sub>W_all_struct_inv_def cdcl\<^sub>W_M_level_inv_def
-    by fast
-
-  show ?thesis
-  proof (cases \<open>count_decided (trail S) = 0\<close>)
-    case True
-    have \<open>get_all_ann_decomposition (trail S) = [([], trail S)]\<close>
-      apply (rule no_decision_get_all_ann_decomposition)
-      using True by (auto simp: count_decided_0_iff)
-    then show ?thesis
-      using decomp L_trail
-      unfolding all_decomposition_implies_def
-      by (auto intro: true_clss_clss_in_imp_true_clss_cls)
-  next
-    case False
-    then obtain K M1 M2 M3 where
-      decomp': \<open>(Decided K # M1, M2) \<in> set (get_all_ann_decomposition (trail S))\<close> and
-      lev_K: \<open>get_level (trail S) K = Suc 0\<close> and
-      M3: \<open>trail S = M3 @ M2 @ Decided K # M1\<close>
-      using struct_invs backtrack_ex_decomp[of S 0] unfolding cdcl\<^sub>W_all_struct_inv_def by blast
-    then have dec_M1: \<open>count_decided M1 = 0\<close>
-      using n_d by auto
-    define M2' where \<open>M2' = M3 @ M2\<close>
-    then have M3: \<open>trail S = M2' @ Decided K # M1\<close> using M3 by auto
-    have \<open>get_all_ann_decomposition M1 = [([], M1)]\<close>
-      apply (rule no_decision_get_all_ann_decomposition)
-      using dec_M1 by (auto simp: count_decided_0_iff)
-    then have \<open>([], M1) \<in> set (get_all_ann_decomposition (trail S))\<close>
-      using hd_get_all_ann_decomposition_skip_some[of Nil M1 M1 \<open>_ @ _\<close>] decomp'
-      by auto
-    then have \<open>set_mset (clauses S) \<Turnstile>ps unmark_l M1\<close>
-      using decomp
-      unfolding all_decomposition_implies_def by auto
-    moreover {
-      have \<open>L \<in> lits_of_l M1\<close>
-        using n_d lev M3 in_trail
-        by (cases \<open>undefined_lit (M2' @ Decided K # []) L\<close>) (auto dest: in_lits_of_l_defined_litD)
-      then have \<open>{#L#} \<in> unmark_l M1\<close>
-        using in_trail by (auto simp: in_unmark_l_in_lits_of_l_iff)
-    }
-    ultimately show ?thesis
-      unfolding all_decomposition_implies_def
-      by (auto intro: true_clss_clss_in_imp_true_clss_cls)
-  qed
-qed
-end
-
-(* TODO Move *)
-lemma subseteq_remove1[simp]: \<open>C \<subseteq># C' \<Longrightarrow> remove1_mset L C \<subseteq># C'\<close>
-  by (meson diff_subset_eq_self subset_mset.dual_order.trans)
-(* End Move *)
-
 lemma lit_redundant_rec_spec:
   fixes L :: \<open>'v literal\<close>
   assumes invs: \<open>cdcl\<^sub>W_restart_mset.cdcl\<^sub>W_all_struct_inv (M, N + NP, U + UP, D')\<close>
@@ -1754,13 +1681,21 @@ definition cach_refinement
 where
   \<open>cach_refinement = cach_refinement_nonull O cach_refinement_list\<close>
 
+lemma cach_refinement_alt_def:
+  \<open>cach_refinement = {((cach, support), cach').
+       (\<forall>L < length cach. cach ! L \<noteq> SEEN_UNKNOWN \<longrightarrow> L \<in> set support) \<and>
+       (\<forall>L \<in> set support. L < length cach) \<and>
+       (\<forall>L \<in># \<A>\<^sub>i\<^sub>n. L < length cach \<and> cach ! L = cach' L)}\<close>
+  unfolding cach_refinement_def cach_refinement_nonull_def cach_refinement_list_def
+  by (auto simp: map_fun_rel_def)
+
 abbreviation (in -) cach_refinement_l_assn where
   \<open>cach_refinement_l_assn \<equiv> array_assn minimize_status_assn *a arl_assn uint32_nat_assn\<close>
 
 definition cach_refinement_assn where
   \<open>cach_refinement_assn = hr_comp cach_refinement_l_assn cach_refinement\<close>
 
-lemma cach_refinement_alt_def:
+lemma in_cach_refinement_alt_def:
   \<open>((cach, support), cach') \<in> cach_refinement \<longleftrightarrow>
      (cach, cach') \<in> cach_refinement_list \<and>
      (\<forall>L<length cach. cach ! L \<noteq> SEEN_UNKNOWN \<longrightarrow> L \<in> set support) \<and>
