Weidenbach_Book/CDCL_W_Abstract_State.thy
@@ -217,4 +217,16 @@ next
   qed
 qed
 
+
+lemma full_cdcl\<^sub>W_init_state:
+  \<open>full cdcl\<^sub>W_restart_mset.cdcl\<^sub>W_stgy (init_state {#}) S \<longleftrightarrow> S = init_state {#}\<close>
+  unfolding full_def rtranclp_unfold
+  by (subst tranclp_unfold_begin)
+     (auto simp:  cdcl\<^sub>W_restart_mset.cdcl\<^sub>W_stgy.simps
+      cdcl\<^sub>W_restart_mset.conflict.simps cdcl\<^sub>W_restart_mset.cdcl\<^sub>W_o.simps
+       cdcl\<^sub>W_restart_mset.propagate.simps cdcl\<^sub>W_restart_mset.decide.simps
+       cdcl\<^sub>W_restart_mset.cdcl\<^sub>W_bj.simps cdcl\<^sub>W_restart_mset.backtrack.simps
+      cdcl\<^sub>W_restart_mset.skip.simps cdcl\<^sub>W_restart_mset.resolve.simps
+      cdcl\<^sub>W_restart_mset_state clauses_def)
+
 end
