Weidenbach_Book/Two_Watched_Literals_List.thy
@@ -73,6 +73,7 @@ lemma convert_lits_l_cons[simp]: \<open>convert_lits_l N (L # M) = convert_lit N
 lemma convert_lits_l_append[simp]: \<open>convert_lits_l N (M @ M') = convert_lits_l N M @ convert_lits_l N M'\<close>
   by (auto simp: convert_lits_l_def)
 
+
 fun get_learned_l :: "'v twl_st_l \<Rightarrow> nat" where
   \<open>get_learned_l (_, _, U, _, _, _, _, _) = U\<close>
 
@@ -151,6 +152,14 @@ lemma get_level_convert_lits_l[simp]: \<open>get_level (convert_lits_l N M) = ge
   apply (rule ext)
   by (induction M) (auto simp: get_level_def convert_lits_l_def)
 
+lemma get_level_convert_lits_l2[simp]:
+  \<open>get_level (convert_lits_l N M') K = get_level M' K\<close>
+  using get_level_convert_lits_l[of N M'] by simp
+
+lemma hd_get_trail_twl_st_of_get_trail_l:
+  \<open>get_trail_l S \<noteq> [] \<Longrightarrow> lit_of (hd (get_trail (twl_st_of None S))) = lit_of (hd (get_trail_l S))\<close>
+  by (cases S; cases \<open>get_trail_l S\<close>) auto
+
 lemma count_decided_convert_lits_l[simp]:
   \<open>count_decided (convert_lits_l N M) = count_decided M\<close>
   by (auto simp: count_decided_def convert_lits_l_def)
@@ -216,8 +225,8 @@ lemma polarity_None_undefined_lit: \<open>is_None (polarity M L) \<Longrightarro
 lemma polarity_spec:
   assumes \<open>no_dup M\<close>
   shows
-  \<open>RETURN (polarity M L) \<le> SPEC(\<lambda>v. (v = None \<longleftrightarrow> undefined_lit M L) \<and>
-    (v = Some True \<longleftrightarrow> L \<in> lits_of_l M) \<and> (v = Some False \<longleftrightarrow> -L \<in> lits_of_l M))\<close>
+    \<open>RETURN (polarity M L) \<le> SPEC(\<lambda>v. (v = None \<longleftrightarrow> undefined_lit M L) \<and>
+      (v = Some True \<longleftrightarrow> L \<in> lits_of_l M) \<and> (v = Some False \<longleftrightarrow> -L \<in> lits_of_l M))\<close>
   unfolding polarity_def
   by refine_vcg
     (use assms in \<open>auto simp: defined_lit_map lits_of_def atm_of_eq_atm_of uminus_lit_swap
@@ -1497,15 +1506,6 @@ lemma get_all_ann_decomposition_convert_lits_l:
   subgoal for L m M by (cases \<open>get_all_ann_decomposition M\<close>) auto
   done
 
-(* TODO Move upper  *)
-lemma get_level_convert_lits_l2[simp]:
-  \<open>get_level (convert_lits_l N M') K = get_level M' K\<close>
-  using get_level_convert_lits_l[of N M'] by simp
-
-lemma hd_get_trail_twl_st_of_get_trail_l:
-  \<open>get_trail_l S \<noteq> [] \<Longrightarrow> lit_of (hd (get_trail (twl_st_of None S))) = lit_of (hd (get_trail_l S))\<close>
-  by (cases S; cases \<open>get_trail_l S\<close>) auto
-(* End Move  *)
 
 lemma mset_take_drep_tl_id[simp]:
   \<open>mset (take x1i (tl x1h)) + mset (drop (Suc x1i) x1h) = mset (tl x1h)\<close>
